theories/ExamplePairingHeap.v
@@ -1,8 +1,11 @@
 (**
 
-Formalization of 
-- purely functional pairing heaps in Coq
+Formalization of pairing heaps, covering both
+- purely functional pairing heaps (in Coq code)
 - ephemeral (pointer-based) pairing heaps in CFML2
+
+More information about pairing heaps:
+  https://www.cise.ufl.edu/~sahni/dsaaj/enrich/c13/pairing.htm
 
 Author: Arthur Charguéraud.
 License: MIT.
@@ -10,139 +13,117 @@ License: MIT.
 *)
 
 Set Implicit Arguments.
-From TLC Require Import LibCore.
-From Sep Require Import Example.
-From Sep Require Import ExampleList.
+From TLC Require Import LibCore LibMultiset.
+From Sep Require Import Example ExampleList.
+Module Import M := MList.MListOf.
 
 
-(* ******************************************************* *)
-(** ** Mutable lists extension *)
+(* ********************************************************************** *)
+(* ********************************************************************** *)
+(* ********************************************************************** *)
+(** * Representation and lemmas *)
 
-Module MList.
+(* ********************************************************************** *)
+(** ** Types of elements *)
 
-Definition head : field := 0%nat.
-Definition tail : field := 1%nat.
-
-Fixpoint MListOf A `{EA:Enc A} TA (R:TA->A->hprop) (L:list TA) (p:loc) : hprop :=
-  match L with
-  | nil => \[p = null]
-  | X::L' => \exists x p', p ~> Record`{ head := x; tail := p'} \* (x ~> R X) \* (p' ~> MListOf R L')
-  end.
-
-(*
-  \exists v, p ~~> v \*
-  match L with
-  | nil => \[v = Nil]
-  | x::L' => \exists X p', \[v = Cons x p'] \* (x ~> RA X) \* (p' ~> MList L')
-  end.
-*)
-
-Section Ops.
-
-Context A {EA:Enc A} TA (R:TA->A->hprop).
-Implicit Types L : list TA.
-Implicit Types p : loc.
-Implicit Types x : A.
-Implicit Types X : TA.
-
-Parameter is_empty : val.
-
-Parameter Triple_is_empty : forall L p,
-  TRIPLE (is_empty p)
-    PRE (p ~> MListOf R L)
-    POST (fun b => \[b = isTrue (L = nil)] \* p ~> MListOf R L).
-
-Parameter push : val.
-
-Parameter Triple_push : forall L p x X,
-  TRIPLE (push p ``x)
-    PRE (p ~> MListOf R L \* x ~> R X)
-    POST (fun (_:unit) => p ~> MListOf R (X::L)).
-
-Parameter pop : val.
-
-Parameter Triple_pop : forall L p,
-  L <> nil ->
-  TRIPLE (pop p)
-    PRE (p ~> MListOf R L)
-    POST (fun x => \exists X L', \[L = X::L'] \* x ~> R X \* p ~> MListOf R L').
-
-End Ops.
-
-End MList.
-
-
-(* ####################################################### *)
-
-From TLC Require Import LibMultiset.
-
-Tactic Notation "multiset_eq" := (* TODO: move to TLC *)
-  check_noevar_goal; permut_simpl.
-
-
-
-(** For simplicity, assume the heap stores integer values.
+(** For simplicity, assume the priority queue to store integer values.
     It is not hard to generalize everything to any ordered type. *)
 
 Notation "'elem'" := (int).
 Notation "'elems'" := (multiset elem).
 
 
-(* ####################################################### *)
-(** * Data types and invariants *)
-
-
 (* ******************************************************* *)
-(** ** Data types *)
+(** ** Data structure and definitions *)
 
-Inductive heap : Type :=
-  | Empty : heap
-  | Node : elem -> list heap -> heap.
+(** Functional representation of a node in a (nonempty) pairing heap *)
+
+Inductive node : Type :=
+  | Node : elem -> list node -> node.
+
+Instance Inhab_node : Inhab node.
+Proof using. applys Inhab_of_val (Node arbitrary nil). Qed.
+
+(** Functional representation of a possibly-empty pairing heap *)
+
+Definition heap := option node.
 
 Instance Inhab_heap : Inhab heap.
-Proof using. applys Inhab_of_val Empty. Qed.
+Proof using. applys Inhab_of_val (@None node). Qed.
 
+(** Auxiliary definition for specifications *)
 
-(* ******************************************************* *)
-(** ** Invariant *)
-
-Implicit Types x y : elem.
-Implicit Types h : heap.
-Implicit Types hs : list heap.
-Implicit Types E : elems.
-Implicit Types Es : list elems.
-
-Definition min_of (E:elems) (x:elem) := 
+Definition min_of (E:elems) (x:elem) : Prop := 
   x \in E /\ forall_ y \in E, x <= y.
 
-Definition removed_min (E E':elems) : Prop :=
-  exists x, min_of E x /\ E = \{x} \u E'.
+(** Auxiliary definition for stating invariants follow. *)
+
+(** [is_ge x] is a predicate that characterizes items no less than [x] *)
 
 Definition is_ge (x y:elem) : Prop :=
   x <= y.
 
-Definition list_union (Es:list elems) := 
+(** [list_union Es] computes the iterated union of the multisets in the list [Es] *)
+
+Definition list_union (Es:list elems) : elems := 
   LibList.fold_right union \{} Es.
 
-Inductive inv : heap -> elems -> Prop :=
-  | inv_Empty : 
-      inv Empty \{} 
-  | inv_Node : forall x hs Es E,
-      Forall2 inv hs Es ->
+(** [inv n E] relates a tree node [n] with the multiset [E] made of
+    the items that the tree contains *)
+
+Inductive inv : node -> elems -> Prop :=
+  | inv_Node : forall x ns Es E,
+      Forall2 inv ns Es ->
       Forall (foreach (is_ge x)) Es ->
       E = \{x} \u (list_union Es) ->   
-      inv (Node x hs) E.
+      inv (Node x ns) E.
+
+(** [repr h E] relates a heap representation [h] with the multiset [E] made of the items 
+    that the heap contains *)
+
+Inductive repr : heap -> elems -> Prop :=
+  | repr_None :
+      repr None \{}
+  | repr_Some : forall n E,
+      inv n E ->
+      repr (Some n) E.
 
 
 (* ******************************************************* *)
 (** ** Lemmas and tactics *)
 
+(** Implicit Types *)
+
+Implicit Types n : node.
+Implicit Types p q l : loc.
+Implicit Types x y : elem.
+Implicit Types h : heap.
+Implicit Types hs : list node.
+Implicit Types E : elems.
+Implicit Types Es : list elems.
+
+(** Normalization lemmas for [list_union] *)
+
+Lemma list_union_nil :
+  list_union (@nil elems) = \{}.
+Proof using. auto. Qed.
+
+Lemma list_union_cons : forall E Es,
+  list_union (E::Es) = E \u list_union Es.
+Proof using. auto. Qed.
+
+(** Hints *)
+
+Hint Rewrite list_union_nil list_union_cons : rew_listx.
+Hint Rewrite (@union_empty_r elems _ _ _) (@union_empty_l elems _ _ _) : rew_listx.
 Hint Extern 1 (_ < _) => simpl; math.
 Hint Extern 1 (_ <= _) => simpl; math.
-Hint Extern 1 (_ = _ :> multiset _) => unfold list_union; rew_listx; multiset_eq.
+Hint Extern 1 (_ = _ :> multiset _) => rew_listx; multiset_eq.
 Hint Extern 1 (_ \in (_ : multiset _)) => multiset_in.
 Hint Constructors Forall Forall2 list_sub.
 Hint Unfold is_ge.
+
+(** Lemmas to manipulate the invariant [Forall (foreach (is_ge x)) Es] *)
 
 Lemma Forall_foreach_is_ge_inv : forall x y Es,
   Forall (foreach (is_ge x)) Es ->
@@ -163,13 +144,21 @@ Proof using.
   { unfold list_union; rew_listx. applys* foreach_union. }
 Qed.
 
-Lemma merge_lemma : forall x1 x2 hs1 hs2 Es1 Es2,
-  Forall2 inv hs1 Es1 ->
-  Forall2 inv hs2 Es2 ->
+(** Key auxiliary lemmas for the verification proofs
+    (both for the functional version and the imperative version) *)
+
+Lemma inv_not_empty : forall n E,
+  inv n E ->
+  E <> \{}.
+Proof using. introv I. inverts I. multiset_inv. Qed.
+
+Lemma merge_lemma : forall x1 x2 ns1 ns2 Es1 Es2,
+  Forall2 inv ns1 Es1 ->
+  Forall2 inv ns2 Es2 ->
   Forall (foreach (is_ge x2)) Es1 ->
   Forall (foreach (is_ge x1)) Es2 ->
   x1 <= x2 ->
-  inv (Node x1 (Node x2 hs1 :: hs2)) ('{x1} \u '{x2} \u list_union Es1 \u list_union Es2).
+  inv (Node x1 (Node x2 ns1 :: ns2)) ('{x1} \u '{x2} \u list_union Es1 \u list_union Es2).
 Proof using.
   introv Is1 Is2 Ks1 Ks2 L. applys_eq inv_Node 1. constructor.
   { applys* inv_Node. }
@@ -191,50 +180,61 @@ Proof.
   introv M. split. 
   { auto. }
   { intros y Hy. multiset_in Hy.
-    { auto. }  { applys* Forall_foreach_is_ge_inv Es. } }
+    { auto. } { applys* Forall_foreach_is_ge_inv Es. } }
 Qed.
 
 
-(* ####################################################### *)
+(* ********************************************************************** *)
+(* ********************************************************************** *)
+(* ********************************************************************** *)
 (** * Purely functional pairing heaps *)
 
-Module PurePairing.
+Module Pure.
 
 (* ******************************************************* *)
-(** ** Coq code *)
+(** ** Source code *)
 
 Definition empty : heap :=
-  Empty.
+  None.
 
 Definition is_empty (h:heap) : bool :=
   match h with
-  | Empty => true
+  | None => true
   | _ => false
   end.
 
-Definition merge (h1 h2:heap) : heap :=
-  match h1, h2 with
-   | _, Empty => h1
-   | Empty, _ => h2
-   | Node x hs1, Node y hs2 =>
-       If x < y
-          then Node x (h2::hs1)
-          else Node y (h1::hs2)
-   end.
+Definition merge (n1 n2:node) : node :=
+  match n1, n2 with Node x ns1, Node y ns2 =>
+     If x < y
+        then Node x (n2::ns1)
+        else Node y (n1::ns2)
+  end.
 
 Definition insert (h:heap) (x:elem) : heap :=
-  merge (Node x nil) h.
+  let n' := Node x nil in
+  match h with
+  | None => Some n'
+  | Some n => Some (merge n n')
+  end.
 
-Fixpoint merge_pairs (hs:list heap) : heap :=
-  match hs with
-  | nil => Empty
-  | h::nil => h
-  | h1::h2::hs' => merge (merge h1 h2) (merge_pairs hs')
+Fixpoint merge_pairs (ns:list node) : node :=
+  match ns with
+  | nil => arbitrary
+  | n::nil => n
+  | n1::n2::hs' => 
+      let n12 := merge n1 n2 in
+      if is_nil hs' 
+        then n12 
+        else merge n12 (merge_pairs hs')
   end.
 
 Definition pop_min (h:heap) : elem * heap :=
   match h with
-  | Node x hs => (x, merge_pairs hs)
+  | Some (Node x ns) =>
+      let h' := if is_nil ns 
+                  then None
+                  else Some (merge_pairs ns) in
+      (x, h')
   | _ => arbitrary
   end.
 
@@ -243,139 +243,135 @@ Definition pop_min (h:heap) : elem * heap :=
 (** ** Verification *)
 
 Lemma empty_spec : 
-  inv empty \{}.
+  repr empty \{}.
 Proof using. constructor. Qed.
 
 Lemma is_empty_spec : forall h E,
-  inv h E ->
+  repr h E ->
   is_empty h = isTrue (E = \{}).
 Proof using.
-  introv I. unfold is_empty. destruct h; rew_bool_eq; inverts I.
+  introv I. unfold is_empty. destruct h; rew_bool_eq; inverts I as.
+  { introv N. inverts N. multiset_inv. }
   { auto. }
-  { multiset_inv. }
 Qed.
 
-Lemma merge_spec : forall h1 E1 h2 E2,
-  inv h1 E1 ->
-  inv h2 E2 ->
-  inv (merge h1 h2) (E1 \u E2).
+Lemma merge_spec : forall n1 E1 n2 E2,
+  inv n1 E1 ->
+  inv n2 E2 ->
+  inv (merge n1 n2) (E1 \u E2).
 Proof using.
   introv I1 I2. unfold merge.
-  (destruct h1 as [|x1 hs1]; inverts I1 as; [ intros | intros Is1 Ks1]);
-  (destruct h2 as [|x2 hs2]; inverts I2 as; [ intros | intros Is2 Ks2]).
-  { applys* inv_Empty. }
-  { applys* inv_Node. }
-  { applys* inv_Node. }
-  { rename Es into Es1, Es0 into Es2. case_if.
-    { applys_eq* merge_lemma 1. }
-    { applys_eq* merge_lemma 1. } }
+  (destruct n1 as [x1 ns1]; inverts I1 as; intros Is1 Ks1);
+  (destruct n2 as [x2 ns2]; inverts I2 as; intros Is2 Ks2).
+  rename Es into Es1, Es0 into Es2. case_if.
+  { applys_eq* merge_lemma 1. }
+  { applys_eq* merge_lemma 1. }
 Qed.
 
 Lemma insert_spec : forall x h E,
-  inv h E ->
-  inv (insert h x) (E \u \{x}).
+  repr h E ->
+  repr (insert h x) (E \u \{x}).
 Proof using.
-  introv I. unfold insert. applys_eq (>> merge_spec I) 1.
-  { applys* inv_Node. } { autos*. } 
+  introv I. unfold insert.
+  destruct h as [n|].
+  { inverts I as I. constructor. applys_eq (>> merge_spec I) 1.
+    { applys* inv_Node. } { autos*. } } 
+  { inverts I. constructor. applys* inv_Node. }
 Qed.
 
-Lemma merge_pairs_spec : forall hs Es,
-  Forall2 inv hs Es ->
-  inv (merge_pairs hs) (list_union Es).
-Proof using. 
-  intros hs. induction_wf IH: (@LibList.length heap) hs; introv Is.
-  destruct hs as [|h1 hs'']; simpl.
-  { inverts Is. applys inv_Empty. }
-  { inverts Is as I1 Is1. destruct hs'' as [|h2 hs']; simpl.
-    { inverts Is1. unfold list_union. rew_listx. applys_eq~ I1 1. }
-    { inverts Is1 as I2 Is2. rename y into E1, y0 into E2, r0 into Es'.
-      unfold list_union. rew_listx.
-      applys_eq merge_spec 1.
+Lemma merge_pairs_spec : forall ns Es,
+  ns <> nil ->
+  Forall2 inv ns Es ->
+  inv (merge_pairs ns) (list_union Es).
+Proof using.
+  intros ns. induction_wf IH: (@list_sub node) ns; introv N Is.
+  destruct ns as [|n1 ns']; tryfalse. inverts Is as I1 Is. 
+  destruct ns' as [|n2 ns'']; simpl.
+  { inverts Is. rename y into E. applys_eq* I1 1. }
+  { inverts Is as I2 Is. rename r0 into Es, y0 into E2.
+    rewrite is_nil_eq. case_if as C.
+    { subst ns''. inverts Is. applys merge_spec. { applys I1. } { applys_eq* I2 1. } }
+    { applys_eq merge_spec 1.
       { applys* merge_spec. }
-      { applys* IH. hnf; rew_list*. }
+      { applys* IH. }
       { autos*. } } }
 Qed.
 
 Lemma pop_min_spec : forall h E h' x,
   E <> \{} ->
-  inv h E ->
+  repr h E ->
   (x,h') = pop_min h ->
      min_of E x
-  /\ exists E', inv h' E' /\ E = \{x} \u E'.
+  /\ exists E', repr h' E' /\ E = \{x} \u E'.
 Proof using.
   introv N I M. unfolds pop_min.
-  destruct h as [|y hs]; inverts I; tryfalse.
-  { invert M ;=> <- Eh'. forwards* Is: merge_pairs_spec hs. split.
-    { applys* pop_min_lemma. } { eauto. } }
+  destruct h as [n|]; inverts I as I; tryfalse.
+  destruct n as [y ns]. inverts M. inverts I as I1 Ks. split. 
+  { applys~ pop_min_lemma. }
+  { rewrite is_nil_eq. case_if as C.
+    { subst ns. inverts I1. exists \{}. split~. constructor. }
+    { forwards~ Is: merge_pairs_spec I1. exists (list_union Es). split~.
+      constructor~. } }
 Qed.
 
-End PurePairing.
+End Pure.
 
 
+(* ********************************************************************** *)
+(* ********************************************************************** *)
+(* ********************************************************************** *)
+(** * Imperative pairing heaps *)
 
-
-
-(* ####################################################### *)
-(** * Imperative ephemeral pairing heaps *)
-
-
-
-Module ImperativePairing.
-
+Module Imperative.
 
 (* ******************************************************* *)
-(** ** OCaml+null code *)
+(** ** Source code in OCaml+null syntax *)
 
 (**
 [[
 
-  type heap = ref node  (* [ref null] when empty *)
+type node = { value : elem; sub : node mlist }
+type heap = null OR node
 
-  type node = {
-    value : elem;
-    sub : node mlist; }
+let create () =
+  ref null
 
-  let create() =
-    ref null
+let is_empty p = 
+  p == null
 
-	let is_empty h =
-		(!h == null)
+let merge q1 q2 =
+  if q1.value < q2.value 
+    then (MList.push q1.sub q2; q1)
+    else (MList.push q2.sub q1; q2)
 
-  let merge p1 p2 =
-		if p1 == null then p1 else
-		if p2 == null then p2 else
-		if (p1.value < p2.value) then (
-			MList.push p1.sub p2;
-			p1
-		) else (
-			MList.push p2.sub p1;
-			p2
-		)
+let insert p x =
+  let q1 = !p in
+  let q2 = { value = x; sub = MList.create() } in
+  if q1 == null 
+    then p := q2
+    else p := merge q1 q2
 
-  let insert h x =
-    let p = ref { value = x; sub = MList.create() } in
-    h := merge !h p
+let merge_pairs l =
+  let q1 = MList.pop l in
+  if MList.is_empty l then q else
+  let q2 = MList.pop l in
+  let q = merge q1 q2 in
+  if MList.is_empty l 
+     then q
+     else merge q (merge_pairs l)
 
-	let merge_pairs hs =
-    if MList.is_empty hs then null else
-    let h1 = MList.pop hs in
-    if MList.is_empty hs then h1 else
-    let h2 = MList.pop hs in
-		merge (merge h1 h2) (merge_pairs hs)
-
-	let pop_min p =
-    let x = !p.value in
-    p := merge_pairs (!p.sub);
-		x
-
+let pop_min p =
+  let q = !p in
+  let x = q.value in
+  if MList.is_empty q.sub 
+    then p := null
+    else p := merge_pairs q.sub
 ]]
+
 *)
 
-
 (* ******************************************************* *)
-(** ** Deeply embedded code *)
-
-Notation "''hs'" := ("hs":var) : var_scope.
+(** ** Source code in embedded syntax *)
 
 Definition value : field := 0%nat.
 Definition sub : field := 1%nat.
@@ -385,177 +381,252 @@ Definition create : val :=
     val_ref null.
 
 Definition is_empty : val :=
-  VFun 'h := 
-    '!'h '= null.
+  VFun 'p := 
+    '!'p '= null.
 
 Definition merge : val :=
-  VFun 'p1 'p2 := 
-		If_ 'p1 '= null Then 'p1 Else
-		If_ 'p2 '= null Then 'p2 Else
-		If_ ('p1'.value '< 'p2'.value) Then (
-			MList.push ('p1'.sub) 'p2 ';
-			'p1
+  VFun 'q1 'q2 := 
+		If_ ('q1'.value '< 'q2'.value) Then (
+			MList.push ('q1'.sub) 'q2 ';
+			'q1
 		) Else (
-			MList.push ('p2'.sub) 'p1 ';
-			'p2
+			MList.push ('q2'.sub) 'q1 ';
+			'q2
 		).
 
+Definition insert : val :=
+  VFun 'p 'x :=
+    Let 'q1 := '!'p in
+    Let 'q2 := New`{ value := 'x; sub := MList.create '() } in
+    If_ 'q1 '= null
+      Then 'p ':= 'q2
+      Else 'p ':= merge 'q1 'q2.
+
 Definition merge_pairs : val :=
-  VFix 'f 'hs := 
-		If_ MList.is_empty 'hs Then null Else
-    Let 'h1 := MList.pop 'hs in
-    If_ MList.is_empty 'hs Then 'h1 Else
-    Let 'h2 := MList.pop 'hs in
-		merge (merge 'h1 'h2) ('f 'hs).
+  VFix 'f 'l := 
+    Let 'q1 := MList.pop 'l in
+    If_ MList.is_empty 'l Then 'q1 Else
+    Let 'q2 := MList.pop 'l in
+    Let 'q := merge 'q1 'q2 in
+		If_ MList.is_empty 'l Then 'q Else
+    merge 'q ('f 'l).
 
 Definition pop_min : val :=
   VFun 'p :=
-    Let 'x := '!'p'.value in
-    'p ':= merge_pairs ('!'p'.sub) ';
+    Let 'q := '!'p in
+    Let 'x := 'q'.value in
+    (If_ MList.is_empty ('q'.sub)
+      Then 'p ':= null
+      Else 'p ':= merge_pairs ('q'.sub) )';
 		'x.
 
 
-
 (* ******************************************************* *)
-(** ** Representation predicate *)
+(** ** Representation predicates *)
 
-(*
-Definition Heap (E:elems) (p:loc) : hprop :=
-  \exists (v:loc), p ~~> v \*
-  If E = \{} then \[v = null] else 
-    \exists x hs, v ~> Record`{ value := x; sub := hs } \* .
-*)
-(*
-Inductive tree : Type :=
-  | Leaf : tree
-  | Node : list tree -> tree.
+(** [q ~> Tree n] related a pointer [q] with the functional tree structure [n]
+    that it represents in memory *)
 
-Fixpoint MListOf' A TA (R:TA->A->hprop) (L:list TA) (p:loc) : hprop :=
-  match L with
-  | nil => \[p = null]
-  | X::L' => (p ~> MListOf' R L')
-  end.
-
-
-Fixpoint Repr (t:tree) (p:loc) {struct t} :=
-  match t with
-  | Leaf => \[p = null]
-  | Node ts => (* MListOf' Repr ts p*)
-    (fix f R ts p : hprop := match ts with
-    | nil => \[p = null]
-    | X::L' => (p ~> f R L') \* p ~> R X
-    end) Repr ts p
-  end.
-
-
-      Fixpoint MListOf' A TA (R:TA->A->hprop) (L:list TA) (p:loc) : hprop :=
-  match L with
-  | nil => \[p = null]
-  | X::L' => (p ~> MListOf' R L')
-  end.
-
-Fixpoint MListOf A `{EA:Enc A} TA (R:TA->A->hprop) (L:list TA) (p:loc) : hprop :=
-  match L with
-  | nil => \[p = null]
-  | X::L' => \exists x p', p ~> Record`{ head := x; tail := p'} \* (x ~> R X) \* (p' ~> MListOf R L')
-  end.
-
-Fixpoint MListOf' A `{EA:Enc A} TA (R:TA->A->hprop) (L:list TA) (p:loc) : hprop :=
-  match L with
-  | nil => \[p = null]
-  | X::L' => \exists (x:A) p', p ~> Record`{ head := x; tail := p'} \* (x ~> R X) \* (p' ~> MListOf' R L')
-  end.
-*)
-
-Definition head : field := 0%nat.
-Definition tail : field := 1%nat.
-
-
-
-Fixpoint Repr (h:heap) (p:loc) { struct h } : hprop :=
-  match h with
-  | Empty => \[p = null]
+Fixpoint Tree (n:node) (q:loc) { struct n } : hprop :=
+  match n with
   | Node x hs => 
-      \exists q,
-       p ~> Record`{ value := x; sub := q } 
-      (* \* q ~> MListOf Repr hs *) \*
-      (fix MListOf L p : hprop :=
-      match L with
-      | nil => \[p = null]
-      | X::L' => \exists (x:loc) p', p ~> Record`{ head := x; tail := p'} \* (x ~> Repr X) \* (p' ~> MListOf L')
-      end) hs q
+      \exists (q':loc),
+         q ~> Record`{ value := x; sub := q' } 
+      \* q' ~> M.MListOf Tree hs
   end.
 
-Lemma Repr_eq : forall h p,
-    Repr h p 
-  = match h with
-    | Empty => \[p = null]
-    | Node x hs => 
-        \exists q,
-         p ~> Record`{ value := x; sub := q } 
-       \* q ~> MList.MListOf Repr hs
-   end.
-Proof using.
-  intros. gen p. induction h; intros.
-  auto.
-  simpl.
-  fequals. applys fun_ext_1.  intros q. fequals. gen q. induction l; intros.
-  auto.
-  simpl. xrepr_clean.  fequals.   applys fun_ext_1.  intros x. fequals. 
-applys fun_ext_1.  intros p'. fequals. fequals.
-Admitted. (* generalized induction on trees *)
+(** [q ~> Repr E] related a non-null pointer [q] with the multiset of items [E]
+    that are stored in the tree *)
 
+Definition Repr (E:elems) (q:loc) : hprop :=
+  \exists n, q ~> Tree n \* \[inv n E].
 
+(** [q ~> Heap E] relates a possibly-null pointer [q] with the multiset of items [E]
+    that are stored in the heap. It uses [Contents E q] as an auxiliary definition. *)
+
+Definition Contents (E:elems) (q:loc) : hprop :=
+  If q = null then \[E = \{}] else q ~> Repr E.
 
 Definition Heap (E:elems) (p:loc) : hprop :=
-  \exists (h:heap), p ~> Repr h \* \[inv h E].
-
+  \exists q, p ~~> q \* Contents E q.
 
 
 (* ******************************************************* *)
-(** ** Verification 
+(** ** Lemmas for the representation predicates *)
 
+(** For [Tree] *)
 
-Lemma triple_create :
-  triple (val_create val_unit)
-    \[]
-    (fun r => \exists p, \[r = val_loc p] \* MQueue nil p).
+Lemma Tree_Node : forall q x hs,
+  q ~> Tree (Node x hs) =
+      \exists l, q ~> Record`{ value := x; sub := l }
+              \* l ~> M.MListOf Tree hs.
+Proof using. auto. Qed.
+
+(** For [Repr] *)
+
+Lemma Repr_eq : forall q E,
+  q ~> Repr E = \exists n, q ~> Tree n \* \[inv n E].
+Proof using. auto. Qed.
+
+Lemma Repr_not_empty : forall q E,
+  q ~> Repr E ==> \[E <> \{}] \* q ~> Repr E.
 Proof using.
-  xcf. unfold MQueue.
-  xapp triple_alloc_cell as r. intros p v1 v2. intro_subst.
-  xapp~. xpull ;=> r x E. xsimpl~.
-  { rewrite MListSeg_nil_eq. xsimpl~. }
+  intros. xunfold Repr. xpull ;=> n I. lets: inv_not_empty I. xsimpl*.
 Qed.
 
-*)
-
-(* ####################################################### *)
-
-(* LATER: transitive closure of sublist (tclosure (@list_sub heap)) *)
-(* FOR TLC
-Hint Resolve wf_tclosure : wf.
-
-
-Lemma Forall_foreach_pred_incl : forall P Q Es,
-  Forall (foreach P) Es ->
-  pred_incl P Q ->
-  Forall (foreach Q) Es.
+Lemma Repr_not_null : forall q E,
+  q ~> Repr E ==> \[q <> null] \* q ~> Repr E.
 Proof using.
-  introv M N. applys Forall_pred_incl M. intros x Hx.
-  applys* foreach_weaken. (* LATER: foreach_pred_incl. *)
+  intros. xunfold Repr. xpull ;=> n I. destruct n as [x hs].
+  rewrite Tree_Node. xpull ;=> l. xchange* Record_not_null ;=> N.
+  xsimpl~ (Node x hs). rewrite Tree_Node. xsimpl.
 Qed.
-*)
+
+(** For [Contents] *)
+
+Lemma Contents_eq : forall E q,
+  Contents E q = (If q = null then \[E = \{}] else q ~> Repr E).
+Proof using. auto. Qed.
+
+Lemma Contents_not_empty : forall E q,
+  E <> \{} ->
+  Contents E q = (q ~> Repr E).
+Proof using.
+  introv N. unfold Contents. applys himpl_antisym.
+  { case_if; xsimpl. }
+  { xchange Repr_not_null ;=> N'. case_if*. }
+Qed.
+
+Lemma Contents_is_empty : forall q E,
+  Contents E q ==> \[q = null <-> E = \{}] \* Contents E q.
+Proof using.
+  intros. unfold Contents. case_if.
+  { xsimpl*. } 
+  { xchange Repr_not_empty ;=> N. xsimpl*. }
+Qed.
+
+Lemma Contents_null :
+  \[] ==> Contents \{} null.
+Proof using. unfold Contents. case_if. xsimpl*. Qed.
+
+(** For [Heap] *)
+
+Lemma Heap_eq : forall p E,
+  p ~> Heap E = \exists q, p ~~> q \* Contents E q.
+Proof using. auto. Qed.
+
+Lemma Heap_of_Repr : forall p q E,
+  p ~~> q \* q ~> Repr E ==> p ~> Heap E.
+Proof using.
+  intros. xchanges Repr_not_empty ;=> N. xunfold Heap.
+  xsimpl. xchange Repr_not_null ;=> N'. unfold Contents. case_if~.
+Qed.
+
+Lemma Heap_of_null : forall p,
+  p ~~> null ==> p ~> Heap \{}.
+Proof using. intros. xchanges Contents_null. xchange <- Heap_eq. Qed.
 
 
-(*
+(* ******************************************************* *)
+(** ** Verification *)
 
-https://sites.google.com/site/progyumming/cpp/pairing-heap
+Lemma Triple_create :
+  TRIPLE (create tt)
+    PRE \[]
+    POST (fun p => p ~> Heap \{}).
+Proof using.
+  xwp. xapp (>> Triple_ref Enc_loc null) ;=> p.
+  xunfold Heap. xsimpl. xchanges~ Contents_null.
+Qed.
 
-https://github.com/saadtaame/pairing-heap/blob/master/pairing_heap.cc
+Hint Extern 1 (Register_Spec (create)) => Provide @Triple_create.
 
-https://www.sanfoundry.com/cpp-program-implement-pairing-heap/
+Lemma Triple_is_empty : forall p E,
+  TRIPLE (is_empty p)
+    PRE (p ~> Heap E)
+    POST (fun b => \[b = isTrue (E = \{})] \* p ~> Heap E).
+Proof using.
+  xwp. xunfolds Heap ;=> q. xapp. xapp. typeclass.
+  xchanges~ Contents_is_empty.
+Qed.
 
-https://www.techiedelight.com/deletion-from-bst/
+Hint Extern 1 (Register_Spec (is_empty)) => Provide @Triple_is_empty.
+
+Lemma Triple_merge : forall q1 q2 E1 E2,
+  TRIPLE (merge q1 q2)
+    PRE (q1 ~> Repr E1 \* q2 ~> Repr E2)
+    POST (fun q => q ~> Repr (E1 \u E2)).
+Proof using.
+  xwp. xchange (Repr_eq q1) ;=> [x1 hs1] I1. xchange (Repr_eq q2) ;=> [x2 hs2] I2.
+  xchange (Tree_Node q1) ;=> l1. xchange (Tree_Node q2) ;=> l2.
+  inverts I1 as Is1 Ks1. inverts I2 as Is2 Ks2.
+  xapp. xapp. xapp. xif ;=> C.
+  { xapp. xchange <- (Tree_Node q2). xapp (>> __ Enc_loc).
+    xval. xchange <- Tree_Node. xchange <- Repr_eq.
+    applys* merge_lemma. xsimpl*. }
+  { xapp. xchange <- (Tree_Node q1). xapp (>> __ Enc_loc).
+    xval. xchange <- Tree_Node. xchange <- Repr_eq.
+    applys* merge_lemma. xsimpl*. }
+Qed.
+
+Hint Extern 1 (Register_Spec (merge)) => Provide @Triple_merge.
+
+Lemma Triple_insert : forall p x E,
+  TRIPLE (insert p x)
+    PRE (p ~> Heap E)
+    POST (fun (_:unit) => p ~> Heap (E \u \{x})).
+Proof using.
+  xwp. xchange Heap_eq ;=> q. xapp. xapp (>> __ Tree) ;=> l.
+  xnew (>> x l). skip. (* TODO noduplicates *) intros q2.
+  xchange <- Tree_Node. xchange <- Repr_eq. { applys* inv_Node. }
+  rew_listx. xapp. typeclass. unfold Contents. xif ;=> C; case_if.
+  { xpull ;=> ->. xapp. xchanges* Heap_of_Repr. }
+  { xapp ;=> r. xapp. xchanges* Heap_of_Repr. }
+Qed.
+
+Hint Extern 1 (Register_Spec (insert)) => Provide @Triple_insert.
+
+Lemma Triple_merge_pairs : forall ns l Es,
+  ns <> nil ->
+  Forall2 inv ns Es ->
+  TRIPLE (merge_pairs l)
+    PRE (l ~> MListOf Tree ns)
+    POST (fun q => q ~> Repr (list_union Es)).
+Proof using.
+  intros ns. induction_wf IH: (@list_sub node) ns; introv N Is.
+  xwp. xapp~ ;=> q1 n1 ns' ->. inverts Is as I1 Is. rename r into Es'.
+  xapp (>> __ Tree). xif ;=> C.
+  { subst. inverts Is. rew_listx. xval. xchanges* <- Repr_eq. }
+  { xapp~ ;=> q2 n2 ns'' ->. inverts Is as I2 Is. rename r into Es''.
+    do 2 xchange* <- Repr_eq. xapp ;=> r. xapp (>> __ Tree). xif ;=> C'.
+    { subst. inverts Is. rew_listx. xvals. }
+    { xapp* ;=> r'. xapp ;=> r''. rew_listx. xsimpl*. } }
+Qed.
+
+Hint Extern 1 (Register_Spec (merge_pairs)) => Provide @Triple_merge_pairs.
+
+Lemma Triple_pop_min : forall p E,
+  E <> \{} ->
+  TRIPLE (pop_min p)
+    PRE (p ~> Heap E)
+    POST (fun x => \exists E', \[min_of E x /\ E = \{x} \u E'] \* p ~> Heap E').
+Proof using.
+  introv HE. xwp. xchange Heap_eq ;=> q. xapp. xchange~ Contents_not_empty.
+  xchange Repr_eq ;=> [x hs] I. invert I ;=> ? ? ? ? Is Ks Eq -> -> ->.
+  xchange Tree_Node ;=> l. xapp.
+  xseq. xapp. xapp (>> __ Tree).
+  xpost (fun (_:unit) => \exists E', \[E = '{x} \u E'] \* p ~> Heap E' \* \GC). xif ;=> C.
+  { { subst. inverts Is. inverts Ks. rew_listx.
+      xapp (>> Triple_set Enc_loc). xchange <- Tree_Node. xchanges* Heap_of_null. } }
+    { xapp. xapp; eauto ;=> r. xapp. xchange Heap_of_Repr. xsimpl*. }
+  { intros _. xpull ;=> E' ->. xval. xsimpl. split~.
+    { rewrite Eq. applys~ pop_min_lemma. } }
+Qed.
+
+Hint Extern 1 (Register_Spec (pop_min)) => Provide @Triple_pop_min.
+
+End Imperative.
 
 
-*)
+
+
