extra/VariantPairingHeap.v
@@ -1,0 +1,561 @@
+(**
+
+Formalization of 
+- purely functional pairing heaps in Coq
+- ephemeral (pointer-based) pairing heaps in CFML2
+
+Author: Arthur Charguéraud.
+License: MIT.
+
+*)
+
+Set Implicit Arguments.
+From TLC Require Import LibCore.
+From Sep Require Import Example.
+From Sep Require Import ExampleList.
+
+
+(* ******************************************************* *)
+(** ** Mutable lists extension *)
+
+Module MList.
+
+Definition head : field := 0%nat.
+Definition tail : field := 1%nat.
+
+Fixpoint MListOf A `{EA:Enc A} TA (R:TA->A->hprop) (L:list TA) (p:loc) : hprop :=
+  match L with
+  | nil => \[p = null]
+  | X::L' => \exists x p', p ~> Record`{ head := x; tail := p'} \* (x ~> R X) \* (p' ~> MListOf R L')
+  end.
+
+(*
+  \exists v, p ~~> v \*
+  match L with
+  | nil => \[v = Nil]
+  | x::L' => \exists X p', \[v = Cons x p'] \* (x ~> RA X) \* (p' ~> MList L')
+  end.
+*)
+
+Section Ops.
+
+Context A {EA:Enc A} TA (R:TA->A->hprop).
+Implicit Types L : list TA.
+Implicit Types p : loc.
+Implicit Types x : A.
+Implicit Types X : TA.
+
+Parameter is_empty : val.
+
+Parameter Triple_is_empty : forall L p,
+  TRIPLE (is_empty p)
+    PRE (p ~> MListOf R L)
+    POST (fun b => \[b = isTrue (L = nil)] \* p ~> MListOf R L).
+
+Parameter push : val.
+
+Parameter Triple_push : forall L p x X,
+  TRIPLE (push p ``x)
+    PRE (p ~> MListOf R L \* x ~> R X)
+    POST (fun (_:unit) => p ~> MListOf R (X::L)).
+
+Parameter pop : val.
+
+Parameter Triple_pop : forall L p,
+  L <> nil ->
+  TRIPLE (pop p)
+    PRE (p ~> MListOf R L)
+    POST (fun x => \exists X L', \[L = X::L'] \* x ~> R X \* p ~> MListOf R L').
+
+End Ops.
+
+End MList.
+
+
+(* ####################################################### *)
+
+From TLC Require Import LibMultiset.
+
+Tactic Notation "multiset_eq" := (* TODO: move to TLC *)
+  check_noevar_goal; permut_simpl.
+
+
+
+(** For simplicity, assume the heap stores integer values.
+    It is not hard to generalize everything to any ordered type. *)
+
+Notation "'elem'" := (int).
+Notation "'elems'" := (multiset elem).
+
+
+(* ####################################################### *)
+(** * Data types and invariants *)
+
+
+(* ******************************************************* *)
+(** ** Data types *)
+
+Inductive heap : Type :=
+  | Empty : heap
+  | Node : elem -> list heap -> heap.
+
+Instance Inhab_heap : Inhab heap.
+Proof using. applys Inhab_of_val Empty. Qed.
+
+
+(* ******************************************************* *)
+(** ** Invariant *)
+
+Implicit Types x y : elem.
+Implicit Types h : heap.
+Implicit Types hs : list heap.
+Implicit Types E : elems.
+Implicit Types Es : list elems.
+
+Definition min_of (E:elems) (x:elem) := 
+  x \in E /\ forall_ y \in E, x <= y.
+
+Definition removed_min (E E':elems) : Prop :=
+  exists x, min_of E x /\ E = \{x} \u E'.
+
+Definition is_ge (x y:elem) : Prop :=
+  x <= y.
+
+Definition list_union (Es:list elems) := 
+  LibList.fold_right union \{} Es.
+
+Inductive inv : heap -> elems -> Prop :=
+  | inv_Empty : 
+      inv Empty \{} 
+  | inv_Node : forall x hs Es E,
+      Forall2 inv hs Es ->
+      Forall (foreach (is_ge x)) Es ->
+      E = \{x} \u (list_union Es) ->   
+      inv (Node x hs) E.
+
+
+(* ******************************************************* *)
+(** ** Lemmas and tactics *)
+
+Hint Extern 1 (_ < _) => simpl; math.
+Hint Extern 1 (_ <= _) => simpl; math.
+Hint Extern 1 (_ = _ :> multiset _) => unfold list_union; rew_listx; multiset_eq.
+Hint Extern 1 (_ \in (_ : multiset _)) => multiset_in.
+Hint Constructors Forall Forall2 list_sub.
+Hint Unfold is_ge.
+
+Lemma Forall_foreach_is_ge_inv : forall x y Es,
+  Forall (foreach (is_ge x)) Es ->
+  y \in list_union Es ->
+  x <= y.
+Proof using. 
+  introv M Hy. unfolds list_union. induction M; rew_listx in *.
+  { multiset_in Hy. }
+  { multiset_in Hy. { applys* H. } { applys* IHM. } }
+Qed.
+
+Lemma foreach_list_union : forall P Es,
+  Forall (foreach P) Es ->
+  foreach P (list_union Es).
+Proof using.
+  introv M. induction M.
+  { applys foreach_empty. }
+  { unfold list_union; rew_listx. applys* foreach_union. }
+Qed.
+
+Lemma merge_lemma : forall x1 x2 hs1 hs2 Es1 Es2,
+  Forall2 inv hs1 Es1 ->
+  Forall2 inv hs2 Es2 ->
+  Forall (foreach (is_ge x2)) Es1 ->
+  Forall (foreach (is_ge x1)) Es2 ->
+  x1 <= x2 ->
+  inv (Node x1 (Node x2 hs1 :: hs2)) ('{x1} \u '{x2} \u list_union Es1 \u list_union Es2).
+Proof using.
+  introv Is1 Is2 Ks1 Ks2 L. applys_eq inv_Node 1. constructor.
+  { applys* inv_Node. }
+  { eauto. }
+  { constructors.
+    { applys foreach_union.
+      { applys* foreach_single. }
+      { applys* foreach_list_union. applys Forall_pred_incl Ks1.
+        { intros x Hx. applys* foreach_weaken. { intros y Hy. unfolds* is_ge. } } } }
+    { eauto. } }
+  { reflexivity. }
+  { autos*. }
+Qed.
+
+Lemma pop_min_lemma : forall x Es,
+  Forall (foreach (is_ge x)) Es ->
+  min_of (\{x} \u list_union Es) x.
+Proof.
+  introv M. split. 
+  { auto. }
+  { intros y Hy. multiset_in Hy.
+    { auto. }  { applys* Forall_foreach_is_ge_inv Es. } }
+Qed.
+
+
+(* ####################################################### *)
+(** * Purely functional pairing heaps *)
+
+Module PurePairing.
+
+(* ******************************************************* *)
+(** ** Coq code *)
+
+Definition empty : heap :=
+  Empty.
+
+Definition is_empty (h:heap) : bool :=
+  match h with
+  | Empty => true
+  | _ => false
+  end.
+
+Definition merge (h1 h2:heap) : heap :=
+  match h1, h2 with
+   | _, Empty => h1
+   | Empty, _ => h2
+   | Node x hs1, Node y hs2 =>
+       If x < y
+          then Node x (h2::hs1)
+          else Node y (h1::hs2)
+   end.
+
+Definition insert (h:heap) (x:elem) : heap :=
+  merge (Node x nil) h.
+
+Fixpoint merge_pairs (hs:list heap) : heap :=
+  match hs with
+  | nil => Empty
+  | h::nil => h
+  | h1::h2::hs' => merge (merge h1 h2) (merge_pairs hs')
+  end.
+
+Definition pop_min (h:heap) : elem * heap :=
+  match h with
+  | Node x hs => (x, merge_pairs hs)
+  | _ => arbitrary
+  end.
+
+
+(* ******************************************************* *)
+(** ** Verification *)
+
+Lemma empty_spec : 
+  inv empty \{}.
+Proof using. constructor. Qed.
+
+Lemma is_empty_spec : forall h E,
+  inv h E ->
+  is_empty h = isTrue (E = \{}).
+Proof using.
+  introv I. unfold is_empty. destruct h; rew_bool_eq; inverts I.
+  { auto. }
+  { multiset_inv. }
+Qed.
+
+Lemma merge_spec : forall h1 E1 h2 E2,
+  inv h1 E1 ->
+  inv h2 E2 ->
+  inv (merge h1 h2) (E1 \u E2).
+Proof using.
+  introv I1 I2. unfold merge.
+  (destruct h1 as [|x1 hs1]; inverts I1 as; [ intros | intros Is1 Ks1]);
+  (destruct h2 as [|x2 hs2]; inverts I2 as; [ intros | intros Is2 Ks2]).
+  { applys* inv_Empty. }
+  { applys* inv_Node. }
+  { applys* inv_Node. }
+  { rename Es into Es1, Es0 into Es2. case_if.
+    { applys_eq* merge_lemma 1. }
+    { applys_eq* merge_lemma 1. } }
+Qed.
+
+Lemma insert_spec : forall x h E,
+  inv h E ->
+  inv (insert h x) (E \u \{x}).
+Proof using.
+  introv I. unfold insert. applys_eq (>> merge_spec I) 1.
+  { applys* inv_Node. } { autos*. } 
+Qed.
+
+Lemma merge_pairs_spec : forall hs Es,
+  Forall2 inv hs Es ->
+  inv (merge_pairs hs) (list_union Es).
+Proof using. 
+  intros hs. induction_wf IH: (@LibList.length heap) hs; introv Is.
+  destruct hs as [|h1 hs'']; simpl.
+  { inverts Is. applys inv_Empty. }
+  { inverts Is as I1 Is1. destruct hs'' as [|h2 hs']; simpl.
+    { inverts Is1. unfold list_union. rew_listx. applys_eq~ I1 1. }
+    { inverts Is1 as I2 Is2. rename y into E1, y0 into E2, r0 into Es'.
+      unfold list_union. rew_listx.
+      applys_eq merge_spec 1.
+      { applys* merge_spec. }
+      { applys* IH. hnf; rew_list*. }
+      { autos*. } } }
+Qed.
+
+Lemma pop_min_spec : forall h E h' x,
+  E <> \{} ->
+  inv h E ->
+  (x,h') = pop_min h ->
+     min_of E x
+  /\ exists E', inv h' E' /\ E = \{x} \u E'.
+Proof using.
+  introv N I M. unfolds pop_min.
+  destruct h as [|y hs]; inverts I; tryfalse.
+  { invert M ;=> <- Eh'. forwards* Is: merge_pairs_spec hs. split.
+    { applys* pop_min_lemma. } { eauto. } }
+Qed.
+
+End PurePairing.
+
+
+
+
+
+(* ####################################################### *)
+(** * Imperative ephemeral pairing heaps *)
+
+
+
+Module ImperativePairing.
+
+
+(* ******************************************************* *)
+(** ** OCaml+null code *)
+
+(**
+[[
+
+  type heap = ref node  (* [ref null] when empty *)
+
+  type node = {
+    value : elem;
+    sub : node mlist; }
+
+  let create() =
+    ref null
+
+	let is_empty h =
+		(!h == null)
+
+  let merge p1 p2 =
+		if p1 == null then p1 else
+		if p2 == null then p2 else
+		if (p1.value < p2.value) then (
+			MList.push p1.sub p2;
+			p1
+		) else (
+			MList.push p2.sub p1;
+			p2
+		)
+
+  let insert h x =
+    let p = ref { value = x; sub = MList.create() } in
+    h := merge !h p
+
+	let merge_pairs hs =
+    if MList.is_empty hs then null else
+    let h1 = MList.pop hs in
+    if MList.is_empty hs then h1 else
+    let h2 = MList.pop hs in
+		merge (merge h1 h2) (merge_pairs hs)
+
+	let pop_min p =
+    let x = !p.value in
+    p := merge_pairs (!p.sub);
+		x
+
+]]
+*)
+
+
+(* ******************************************************* *)
+(** ** Deeply embedded code *)
+
+Notation "''hs'" := ("hs":var) : var_scope.
+
+Definition value : field := 0%nat.
+Definition sub : field := 1%nat.
+
+Definition create : val :=
+  VFun 'u := 
+    val_ref null.
+
+Definition is_empty : val :=
+  VFun 'h := 
+    '!'h '= null.
+
+Definition merge : val :=
+  VFun 'p1 'p2 := 
+		If_ 'p1 '= null Then 'p1 Else
+		If_ 'p2 '= null Then 'p2 Else
+		If_ ('p1'.value '< 'p2'.value) Then (
+			MList.push ('p1'.sub) 'p2 ';
+			'p1
+		) Else (
+			MList.push ('p2'.sub) 'p1 ';
+			'p2
+		).
+
+Definition merge_pairs : val :=
+  VFix 'f 'hs := 
+		If_ MList.is_empty 'hs Then null Else
+    Let 'h1 := MList.pop 'hs in
+    If_ MList.is_empty 'hs Then 'h1 Else
+    Let 'h2 := MList.pop 'hs in
+		merge (merge 'h1 'h2) ('f 'hs).
+
+Definition pop_min : val :=
+  VFun 'p :=
+    Let 'x := '!'p'.value in
+    'p ':= merge_pairs ('!'p'.sub) ';
+		'x.
+
+
+
+(* ******************************************************* *)
+(** ** Representation predicate *)
+
+(*
+Definition Heap (E:elems) (p:loc) : hprop :=
+  \exists (v:loc), p ~~> v \*
+  If E = \{} then \[v = null] else 
+    \exists x hs, v ~> Record`{ value := x; sub := hs } \* .
+*)
+(*
+Inductive tree : Type :=
+  | Leaf : tree
+  | Node : list tree -> tree.
+
+Fixpoint MListOf' A TA (R:TA->A->hprop) (L:list TA) (p:loc) : hprop :=
+  match L with
+  | nil => \[p = null]
+  | X::L' => (p ~> MListOf' R L')
+  end.
+
+
+Fixpoint Repr (t:tree) (p:loc) {struct t} :=
+  match t with
+  | Leaf => \[p = null]
+  | Node ts => (* MListOf' Repr ts p*)
+    (fix f R ts p : hprop := match ts with
+    | nil => \[p = null]
+    | X::L' => (p ~> f R L') \* p ~> R X
+    end) Repr ts p
+  end.
+
+
+      Fixpoint MListOf' A TA (R:TA->A->hprop) (L:list TA) (p:loc) : hprop :=
+  match L with
+  | nil => \[p = null]
+  | X::L' => (p ~> MListOf' R L')
+  end.
+
+Fixpoint MListOf A `{EA:Enc A} TA (R:TA->A->hprop) (L:list TA) (p:loc) : hprop :=
+  match L with
+  | nil => \[p = null]
+  | X::L' => \exists x p', p ~> Record`{ head := x; tail := p'} \* (x ~> R X) \* (p' ~> MListOf R L')
+  end.
+
+Fixpoint MListOf' A `{EA:Enc A} TA (R:TA->A->hprop) (L:list TA) (p:loc) : hprop :=
+  match L with
+  | nil => \[p = null]
+  | X::L' => \exists (x:A) p', p ~> Record`{ head := x; tail := p'} \* (x ~> R X) \* (p' ~> MListOf' R L')
+  end.
+*)
+
+Definition head : field := 0%nat.
+Definition tail : field := 1%nat.
+
+
+
+Fixpoint Repr (h:heap) (p:loc) { struct h } : hprop :=
+  match h with
+  | Empty => \[p = null]
+  | Node x hs => 
+      \exists q,
+       p ~> Record`{ value := x; sub := q } 
+      (* \* q ~> MListOf Repr hs *) \*
+      (fix MListOf L p : hprop :=
+      match L with
+      | nil => \[p = null]
+      | X::L' => \exists (x:loc) p', p ~> Record`{ head := x; tail := p'} \* (x ~> Repr X) \* (p' ~> MListOf L')
+      end) hs q
+  end.
+
+Lemma Repr_eq : forall h p,
+    Repr h p 
+  = match h with
+    | Empty => \[p = null]
+    | Node x hs => 
+        \exists q,
+         p ~> Record`{ value := x; sub := q } 
+       \* q ~> MList.MListOf Repr hs
+   end.
+Proof using.
+  intros. gen p. induction h; intros.
+  auto.
+  simpl.
+  fequals. applys fun_ext_1.  intros q. fequals. gen q. induction l; intros.
+  auto.
+  simpl. xrepr_clean.  fequals.   applys fun_ext_1.  intros x. fequals. 
+applys fun_ext_1.  intros p'. fequals. fequals.
+Admitted. (* generalized induction on trees *)
+
+
+
+Definition Heap (E:elems) (p:loc) : hprop :=
+  \exists (h:heap), p ~> Repr h \* \[inv h E].
+
+
+
+(* ******************************************************* *)
+(** ** Verification 
+
+
+Lemma triple_create :
+  triple (val_create val_unit)
+    \[]
+    (fun r => \exists p, \[r = val_loc p] \* MQueue nil p).
+Proof using.
+  xcf. unfold MQueue.
+  xapp triple_alloc_cell as r. intros p v1 v2. intro_subst.
+  xapp~. xpull ;=> r x E. xsimpl~.
+  { rewrite MListSeg_nil_eq. xsimpl~. }
+Qed.
+
+*)
+
+(* ####################################################### *)
+
+(* LATER: transitive closure of sublist (tclosure (@list_sub heap)) *)
+(* FOR TLC
+Hint Resolve wf_tclosure : wf.
+
+
+Lemma Forall_foreach_pred_incl : forall P Q Es,
+  Forall (foreach P) Es ->
+  pred_incl P Q ->
+  Forall (foreach Q) Es.
+Proof using.
+  introv M N. applys Forall_pred_incl M. intros x Hx.
+  applys* foreach_weaken. (* LATER: foreach_pred_incl. *)
+Qed.
+*)
+
+
+(*
+
+https://sites.google.com/site/progyumming/cpp/pairing-heap
+
+https://github.com/saadtaame/pairing-heap/blob/master/pairing_heap.cc
+
+https://www.sanfoundry.com/cpp-program-implement-pairing-heap/
+
+https://www.techiedelight.com/deletion-from-bst/
+
+
+*)
