extra/hfold.v
@@ -1,0 +1,122 @@
+
+
+Lemma hfold_list_nil : forall f,
+  hfold_list f nil = \[].
+Proof using. auto. Qed.
+(* intros. rewrite hfold_list_eq; unfold hfold_list'. rewrite~ fold_nil. *)
+
+Lemma hfold_list_cons : forall f x l,
+  hfold_list f (x::l) = (f x) \* (hfold_list f l).
+Proof using. auto. Qed.
+(* intros. repeat rewrite hfold_list_eq; unfold hfold_list'. rewrite~ fold_cons. *)
+
+Lemma hfold_list_one : forall f x,
+  hfold_list f (x::nil) = f x.
+Proof using. intros. simpl. xsimpl. Qed.
+(*
+Proof using. intros. rewrite hfold_list_eq; unfold hfold_list'. rewrite~ fold_one. Qed.
+*)
+(*
+
+Lemma hfold_list_app : forall f l1 l2,
+  hfold_list f (l1 ++ l2) = (hfold_list f l1) \* (hfold_list f l2).
+Proof using. intros. repeat rewrite hfold_list_eq; unfold hfold_list'. rewrite~ fold_app. Qed.
+
+Lemma hfold_list_last : forall f x l,
+  hfold_list f (l & x) = (hfold_list f l) \* (f x).
+Proof using. intros. repeat rewrite hfold_list_eq; unfold hfold_list'. rewrite~ fold_last. Qed.
+*)
+
+End HfoldList.
+
+Hint Rewrite hfold_list_nil hfold_list_cons hfold_list_one : rew_heapx.
+(* hfold_list_app hfold_list_last*)
+
+(*
+Definition hfold_list2' A B (f:A->B->hprop) (l1:list A) (l2:list B) : hprop :=
+  hfold_list' (fun '(x1,x2) => f x1 x2) (LibList.combine l1 l2).
+
+-- only for same lengths
+Lemma hfold_list2_eq : 
+  hfold_list2 = hfold_list2'.
+Proof using.
+  unfold hfold_list2', hfold_list'. applys fun_ext_5 ;=> A B f l1.
+  induction l1 as [|x1 l1']; intros l2; destruct l2 as [|x2 l2'].
+  { rewrite . }
+  { unfold hfold_list'. rewrite fold_cons. simpl. rewrite~ IHl'. }
+Qed.
+*)
+
+(* intros. unfold hfold_list2. rew_listx. rewrite~ hfold_list_nil.  *)
+
+
+
+
+=========
+
+
+(* LATER
+Lemma MList_contents_Cons : forall A `{EA:Enc A} (L:list A) x p',
+  (MList_contents (Cons x p') L) ==> \exists L', \[L = x::L'] \* (p' ~> MList L').
+Proof using.
+  intros. unfold MList_contents. destruct L.
+  { xsimpl. }
+  { xpull ;=> p'' E. unfolds @Cons.
+    rewrite (enc_loc_eq p'), (enc_loc_eq p'') in E. (* rew_enc in *. *)
+    asserts_rewrite (x = a). { admit. }
+    (* Enc_injective EA --- all encoders should be injective!  *)
+    inverts E. xsimpl~. }
+Admitted.
+*)
+
+(* ---------------------------------------------------------------------- *)
+(** Detailed proof for set_head *)
+
+(*
+Lemma Triple_set_head' : forall A `{EA:Enc A} (L:list A) p x y,
+  TRIPLE (set_head ``p ``y)
+    PRE (p ~> MList (x::L))
+    POST (fun (_:unit) => p ~> MList (y::L)).
+Proof using.
+  intros. (*  xwp. xgc_post. *) xwp_fun' tt.
+  xchange MList_cons_unfold ;=> q. xapp.
+  applys xcase_lemma0 ;=> E1.
+  { false. }
+  { applys xcase_lemma2.
+    { intros x' q' E. unfold Cons in E. rew_enc in E. inverts E.
+      xval (Cons y q). xapp. xchanges MList_cons. }
+    { intros N. false N. reflexivity. } }
+Qed.
+*)
+
+
+Lemma MListOf_eq : forall A `{EA:Enc A} TA (R:TA->A->hprop) (L:list TA) (p:loc),
+  p ~> MListOf R L =
+  match L with
+  | nil => \[p = null]
+  | X::L' => \exists x p', p ~> Record`{ Field.head := x; Field.tail := p'} 
+                   \* (x ~> R X) \* (p' ~> MListOf R L')
+  end.
+Proof using. intros. xunfold MListOf at 1. destruct~ L. Qed.
+*)
+
+
+(* Bad:
+
+
+Fixpoint MListOf A `{EA:Enc A} TA (R:TA->A->hprop) (L:list TA) (p:loc) : hprop :=
+  match L with
+  | nil => \[p = null]
+  | X::L' => \exists x p', p ~> Record`{ head := x; tail := p'} \* (x ~> R X) \* (p' ~> MListOf R L')
+  end.
+
+Lemma MListOf_eq : forall A `{EA:Enc A} TA (R:TA->A->hprop) (L:list TA) (p:loc),
+  p ~> MListOf R L =
+  match L with
+  | nil => \[p = null]
+  | X::L' => \exists x p', p ~> Record`{ head := x; tail := p'} \* (x ~> R X) \* (p' ~> MListOf R L')
+  end.
+Proof using. intros. xunfold MListOf at 1. destruct~ L. Qed.
+
+
+*)
