theories/TLCbuffer.v
@@ -11,7 +11,7 @@ License: MIT.
 
 Set Implicit Arguments.
 From TLC Require Import LibTactics LibLogic LibList LibReflect.
-From TLC Require LibListZ.
+From TLC Require LibListZ LibWf LibMultiset.
 Generalizable Variables A B.
 
 
@@ -320,7 +320,7 @@ Inductive list_sub : list A -> list A -> Prop :=
 
 Hint Constructors list_sub.
 
-Lemma list_sub_wf : wf list_sub.
+Lemma list_sub_wf : LibWf.wf list_sub.
 Proof using.
   intros l. induction l; apply Acc_intro; introv H.
   { inverts~ H. }
@@ -361,7 +361,7 @@ Definition is_nil A (l:list A) : bool :=
 
 Lemma is_nil_eq : forall A (l:list A),
   is_nil l = isTrue (l = nil).
-Proof using. intros. destruct l; simpl; rew_bool_eq*. Qed.
+Proof using. intros. destruct l; simpl; rew_bool_eq; auto_false. Qed.
 
 Definition is_not_nil A (l:list A) : bool :=
   match l with
@@ -618,7 +618,18 @@ Tactic Notation "list2_ind_last" constr(E) :=
 
 
 (* ---------------------------------------------------------------------- *)
-(* Libmultiset *)
+(* LibMultiset *)
 
 Tactic Notation "multiset_eq" := (* TODO: move to TLC *)
-  check_noevar_goal; permut_simpl.
+  check_noevar_goal; LibMultiset.permut_simpl.
+
+
+(* ---------------------------------------------------------------------- *)
+(* LibList *)
+
+Hint Rewrite fold_nil fold_cons fold_app : rew_listx.
+
+Lemma list_same_length_inv_nil : forall A1 A2 (l1:list A1) (l2:list A2),
+  length l1 = length l2 ->
+  l1 = nil <-> l2 = nil.
+Proof using. intros. destruct l1; destruct l2; auto_false*. Qed.
