theories/WPLifted.v
@@ -785,7 +785,7 @@ Notation "'Let_' [ A EA ] x ':=' F1 'in' F2" :=
 Notation "'Seq' F1 '; F2" :=
   ((Wpgen_seq F1 F2))
   (at level 68, right associativity,
-   format "'[v' 'Seq'  '[' F1 ']' ';  '/'  '[' F2 ']' ']'") : wp_scope.
+   format "'[v' 'Seq'  '[' F1 ']' '';' '/'  '[' F2 ']' ']'") : wp_scope.
 
 Notation "'Letval' x ':=' v 'in' F2" :=
   ((Wpgen_letval_typed v (fun x => F2)))
