export/course_ejcp_2019/README.md
@@ -1,0 +1,38 @@
+#############################################################
+# Version of Coq
+
+The theories compile with Coq 8.8 and they probably also compile 
+with more recent versions. (Let me know otherwise.)
+
+
+
+#############################################################
+# Compilation
+
+
+```
+   git clone https://gitlab.inria.fr/charguer/cfml2_ejcp2019
+   cd cfml2_ejcp2019/theories
+   make
+```
+
+
+#############################################################
+# Interactive session
+
+
+To use CoqIDE, execute:
+
+```
+   ./open.sh
+```
+
+This script executes the following command:
+
+```
+   coqide -async-proofs off -async-proofs-command-error-resilience off EJCPTuto.v EJCPExo.v EJCPImplem.v ExampleStack.v ExampleList.v ExamplePairingHeap.v
+```
+
+The options to CoqIDE makes its use much smoother.
+
+
