export/course_ejcp_2019/extract.sh
@@ -1,0 +1,72 @@
+#!/bin/bash
+
+##############################################################################
+# Configuration
+
+TARGET=~/shared/cfml2_ejcp2019
+THEORIES_TARGET=${TARGET}/theories
+DOC_TARGET=${TARGET}/doc
+
+CFML_FOLDER=~/cfml2/theories
+TLC_FOLDER=~/tlc/src
+DOC_FOLDER=~/cfml2/doc
+
+
+##############################################################################
+# File list
+
+CFML_IMPORTS="Example.v ExampleList.v ExampleStack.v ExamplePairingHeap.v TLCbuffer.v Fmap.v Var.v SepSimpl.v Bind.v Semantics.v SepFunctor.v SepBase.v WPBase.v SepLifted.v WPLifted.v WPTactics.v WPRecord.v WPExamples.v WPExamplesDetails.v WPLib.v EJCPTuto.v EJCPExo.v EJCPImplem.v SLFIntro.v SLFDirect.v SLFExtra.v SLFHprop.v SLFHimpl.v SubstExec.v SLFRules.v SLFWand.v SLFWPsem.v SLFWPgen.v"
+
+TLC_IMPORTS="LibAxioms.v LibTactics.v LibEqual.v LibLogic.v LibOperation.v LibBool.v LibReflect.v LibProd.v LibSum.v LibRelation.v LibOrder.v LibNat.v LibEpsilon.v LibInt.v LibMonoid.v LibContainer.v LibOption.v LibWf.v LibList.v LibListZ.v LibMin.v LibSet.v LibChoice.v LibUnit.v LibCore.v LibFun.v LibFix.v LibMap.v LibString.v LibMultiset.v Makefile.coq"
+
+DOC_IMPORTS="cheatlist.pdf"
+
+
+##############################################################################
+# Create target folder
+
+mkdir -p ${THEORIES_TARGET}
+mkdir -p ${DOC_TARGET}
+
+
+##############################################################################
+# Import local files
+
+cp README.md ${TARGET}
+
+cp Makefile ${THEORIES_TARGET}
+
+cp open.sh ${THEORIES_TARGET}
+
+
+##############################################################################
+# Import CFML
+
+for i in ${CFML_IMPORTS} ; do
+  cp ${CFML_FOLDER}/$i ${THEORIES_TARGET} ;
+done
+
+
+##############################################################################
+# Import TLC
+
+for i in ${TLC_IMPORTS} ; do
+  cp ${TLC_FOLDER}/$i ${THEORIES_TARGET} ;
+done
+
+
+##############################################################################
+# Import DOC
+
+for i in ${DOC_IMPORTS} ; do
+  cp ${DOC_FOLDER}/$i ${DOC_TARGET} ;
+done
+
+
+##############################################################################
+# Remove "From TLC" and "From Sep"
+
+cd ${THEORIES_TARGET}
+sed -i -e 's/^From[[:space:]]TLC[[:space:]]//' *.v
+sed -i -e 's/^From[[:space:]]Sep[[:space:]]//' *.v
+
